WIP on parsers paren-balanced grammar analysis

src/Parsers/Reachable/ParenBalanced/OfParse.v
@@ -6,6 +6,7 @@ Require Import Fiat.Parsers.ContextFreeGrammarProperties.
 Require Import Fiat.Parsers.StringLike.ForallChars.
 Require Import Fiat.Parsers.Reachable.ParenBalanced.Core.
 Require Import Fiat.Parsers.Reachable.ParenBalanced.MinimalOfCore.
+Require Import Fiat.Parsers.Refinement.BinOpBrackets.ParenBalanced.
 Require Import Fiat.Parsers.BaseTypes.
 Require Import Fiat.Parsers.BaseTypesLemmas.
 Require Import Fiat.Common.
@@ -15,40 +16,48 @@ Local Open Scope string_like_scope.
 
 Section cfg.
   Context {Char} {HSL : StringLike Char} {HSLP : StringLikeProperties Char} {G : grammar Char}.
-  Context {predata : parser_computational_predataT}
+  Context {pdata : paren_balanced_hiding_dataT Char}
+          {predata : parser_computational_predataT}
           {rdata' : @parser_removal_dataT' predata}.
 
-  Fixpoint parse_empty_pb_parse_of_productions
+  Fixpoint paren_balanced_pb_parse_of_productions
              {valid0 pats}
-             (str : String) (Hlen : length str = 0) (p : parse_of G str pats)
+             (str : String) (p : parse_of G str pats)
              (Hforall : Forall_parse_of (fun _ nt' => is_valid_nonterminal valid0 nt') p)
+             (Hp : pb'_productions G valid0 pats)
              {struct p}
-  : pb_productions G valid0 pats
-  with parse_empty_pb_parse_of_production
-         {valid0 pat}
-         (str : String) (Hlen : length str = 0) (p : parse_of_production G str pat)
+  : paren_balanced' str 0 = true
+  with paren_balanced_pb_parse_of_production
+         {valid0 pat level}
+         (str : String) (p : parse_of_production G str pat)
          (Hforall : Forall_parse_of_production (fun _ nt' => is_valid_nonterminal valid0 nt') p)
+         (Hp : pb'_production G valid0 level pat)
          {struct p}
-       : pb_production G valid0 pat.
+       : paren_balanced' str level = true.
   Proof.
     { destruct p as [ ?? p | ?? p ]; simpl in *.
-      { pose proof (parse_empty_pb_parse_of_production valid0 _ _ Hlen p Hforall).
-        left; assumption. }
-      { pose proof (parse_empty_pb_parse_of_productions valid0 _ _ Hlen p Hforall).
-        right; assumption. } }
+      { pose proof (fun x => paren_balanced_pb_parse_of_production valid0 _ x str p Hforall) as H'.
+        inversion Hp; subst; clear Hp.
+        apply H'; assumption. }
+      { pose proof (paren_balanced_pb_parse_of_productions valid0 _ str p Hforall) as H'.
+        inversion Hp; subst; clear Hp.
+        apply H'; assumption. } }
     { destruct p as [ | ?? p ]; simpl in *.
-      { constructor. }
-      { constructor.
-        { apply (fun k => @parse_empty_pb_parse_of_item' parse_empty_pb_parse_of_productions valid0 _ _ k _ (fst Hforall)).
+      { rewrite paren_balanced'_nil by assumption.
+        inversion Hp; subst; simpl.
+        reflexivity. }
+      { inversion Hp; subst; clear Hp.
+        { admit; apply (fun k => @paren_balanced_pb_parse_of_item' paren_balanced_pb_parse_of_productions valid0 _ _ k _ (fst Hforall));
           rewrite take_length, Hlen, Min.min_0_r; reflexivity. }
-        { apply (fun k => @parse_empty_pb_parse_of_production valid0 _ _ k _ (snd Hforall)).
+        { pose proof (@paren_balanced_pb_parse_of_production valid0).
+; [ | eassumption ]. x y k). _ (snd Hforall)).
           rewrite drop_length, Hlen; reflexivity. } } }
   Defined.
 
 
 
-  Definition parse_empty_pb_parse_of_item'
-             (parse_empty_pb_parse_of_productions
+  Definition paren_balanced_pb_parse_of_item'
+             (paren_balanced_pb_parse_of_productions
               : forall valid0 pats
                        (str : String) (Hlen : length str = 0) (p : parse_of G str pats)
                        (Hforall : Forall_parse_of (fun _ nt' => is_valid_nonterminal valid0 nt') p),
@@ -61,17 +70,17 @@ Section cfg.
     destruct p as [ | nt p ].
     { exfalso.
       erewrite length_singleton in Hlen by eassumption; omega. }
-    { specialize (parse_empty_pb_parse_of_productions valid0 (G nt) str Hlen p (snd Hforall)).
+    { specialize (paren_balanced_pb_parse_of_productions valid0 (G nt) str Hlen p (snd Hforall)).
       constructor; simpl in *; [ exact (fst Hforall) | assumption ]. }
   Defined.
 
-  Fixpoint parse_empty_pb_parse_of_productions
+  Fixpoint paren_balanced_pb_parse_of_productions
              {valid0 pats}
              (str : String) (Hlen : length str = 0) (p : parse_of G str pats)
              (Hforall : Forall_parse_of (fun _ nt' => is_valid_nonterminal valid0 nt') p)
              {struct p}
   : pb_productions G valid0 pats
-  with parse_empty_pb_parse_of_production
+  with paren_balanced_pb_parse_of_production
          {valid0 pat}
          (str : String) (Hlen : length str = 0) (p : parse_of_production G str pat)
          (Hforall : Forall_parse_of_production (fun _ nt' => is_valid_nonterminal valid0 nt') p)
@@ -79,58 +88,90 @@ Section cfg.
        : pb_production G valid0 pat.
   Proof.
     { destruct p as [ ?? p | ?? p ]; simpl in *.
-      { pose proof (parse_empty_pb_parse_of_production valid0 _ _ Hlen p Hforall).
+      { pose proof (paren_balanced_pb_parse_of_production valid0 _ _ Hlen p Hforall).
         left; assumption. }
-      { pose proof (parse_empty_pb_parse_of_productions valid0 _ _ Hlen p Hforall).
+      { pose proof (paren_balanced_pb_parse_of_productions valid0 _ _ Hlen p Hforall).
         right; assumption. } }
     { destruct p as [ | ?? p ]; simpl in *.
       { constructor. }
       { constructor.
-        { apply (fun k => @parse_empty_pb_parse_of_item' parse_empty_pb_parse_of_productions valid0 _ _ k _ (fst Hforall)).
+        { apply (fun k => @paren_balanced_pb_parse_of_item' paren_balanced_pb_parse_of_productions valid0 _ _ k _ (fst Hforall)).
           rewrite take_length, Hlen, Min.min_0_r; reflexivity. }
-        { apply (fun k => @parse_empty_pb_parse_of_production valid0 _ _ k _ (snd Hforall)).
+        { apply (fun k => @paren_balanced_pb_parse_of_production valid0 _ _ k _ (snd Hforall)).
           rewrite drop_length, Hlen; reflexivity. } } }
   Defined.
 
-  Definition parse_empty_pb_parse_of_item
+  Definition paren_balanced_pb_parse_of_item
              {valid0 it}
              (str : String) (Hlen : length str = 0) (p : parse_of_item G str it)
              (Hforall : Forall_parse_of_item (fun _ nt' => is_valid_nonterminal valid0 nt') p)
   : pb_item G valid0 it
-    := @parse_empty_pb_parse_of_item' (@parse_empty_pb_parse_of_productions) valid0 it str Hlen p Hforall.
+    := @paren_balanced_pb_parse_of_item' (@paren_balanced_pb_parse_of_productions) valid0 it str Hlen p Hforall.
 
-  Definition parse_empty_minimal_pb_parse_of_item
+  Definition paren_balanced_minimal_pb_parse_of_item
              {valid0 it}
              (str : String) (Hlen : length str = 0) (p : parse_of_item G str it)
              (Hforall : Forall_parse_of_item (fun _ nt' => is_valid_nonterminal valid0 nt') p)
   : minimal_pb_item (G := G) valid0 it.
   Proof.
     eapply minimal_pb_item__of__pb_item.
-    eapply parse_empty_pb_parse_of_item; eassumption.
+    eapply paren_balanced_pb_parse_of_item; eassumption.
   Qed.
 
-  Definition parse_empty_minimal_pb_parse_of_production
+  Definition paren_balanced_minimal_pb_parse_of_production
              {valid0 pat}
              (str : String) (Hlen : length str = 0) (p : parse_of_production G str pat)
              (Hforall : Forall_parse_of_production (fun _ nt' => is_valid_nonterminal valid0 nt') p)
   : minimal_pb_production (G := G) valid0 pat.
   Proof.
     eapply minimal_pb_production__of__pb_production.
-    eapply parse_empty_pb_parse_of_production; eassumption.
+    eapply paren_balanced_pb_parse_of_production; eassumption.
   Qed.
 
-  Definition parse_empty_minimal_pb_parse_of_productions
+  Definition paren_balanced_minimal_pb_parse_of_productions
              {valid0 pats}
              (str : String) (Hlen : length str = 0) (p : parse_of G str pats)
              (Hforall : Forall_parse_of (fun _ nt' => is_valid_nonterminal valid0 nt') p)
   : minimal_pb_productions (G := G) valid0 pats.
   Proof.
     eapply minimal_pb_productions__of__pb_productions.
-    eapply parse_empty_pb_parse_of_productions; eassumption.
-  Qed.
+    eapply paren_balanced_pb_parse_of_productions; eassumption.
+  Qed.*)
 
-  Definition parse_empty_from_pb_parse_of_item'
-             (parse_empty_from_pb_parse_of_productions
+  Fixpoint parse_hiding_from_pb_parse_of_productions
+             {valid0 pats}
+             (str : String) (Hlen : length str = 0)
+             (p : pb_productions G valid0 pats)
+             {struct p}
+  : { p : parse_of G str pats
+          & Forall_parse_of (fun _ nt' => is_valid_nonterminal valid0 nt') p }
+  with paren_balanced_from_pb_parse_of_production
+         {valid0 pat}
+         (str : String) (Hlen : length str = 0)
+         (p: pb_production G valid0 pat)
+         {struct p}
+       : { p : parse_of_production G str pat
+               & Forall_parse_of_production (fun _ nt' => is_valid_nonterminal valid0 nt') p }.
+  Proof.
+    { destruct p as [ ?? p | ?? p ]; simpl in *.
+      { pose proof (paren_balanced_from_pb_parse_of_production valid0 _ _ Hlen p) as p'.
+        eexists (ParseHead _ (projT1 p')).
+        exact (projT2 p'). }
+      { pose proof (paren_balanced_from_pb_parse_of_productions valid0 _ _ Hlen p) as p'.
+        eexists (ParseTail _ (projT1 p')).
+        exact (projT2 p'). } }
+    { destruct p as [ | ?? p0 p1 ]; simpl in *.
+      { exists (ParseProductionNil G _ Hlen). constructor. }
+      { eapply (@paren_balanced_from_pb_parse_of_item' paren_balanced_from_pb_parse_of_productions) in p0.
+        eapply (@paren_balanced_from_pb_parse_of_production) in p1.
+        { eexists (ParseProductionCons _ 0 (projT1 p0) (projT1 p1)).
+          exact (projT2 p0, projT2 p1). }
+        { rewrite ?take_length, ?drop_length, Hlen; reflexivity. }
+        { rewrite ?take_length, ?drop_length, Hlen, Min.min_0_r; reflexivity. } } }
+  Defined.
+
+  Definition paren_balanced_from_pb_parse_of_item'
+             (paren_balanced_from_pb_parse_of_productions
               : forall valid0 pats
                        (str : String) (Hlen : length str = 0),
                   pb_productions G valid0 pats
@@ -143,81 +184,49 @@ Section cfg.
           & Forall_parse_of_item (fun _ nt' => is_valid_nonterminal valid0 nt') p }.
   Proof.
     destruct p as [ nt H p ].
-    eapply parse_empty_from_pb_parse_of_productions in p; [ | eassumption.. ].
+    eapply paren_balanced_from_pb_parse_of_productions in p; [ | eassumption.. ].
     exists (ParseNonTerminal _ (projT1 p)).
     exact (H, projT2 p).
   Defined.
 
-  Fixpoint parse_empty_from_pb_parse_of_productions
-             {valid0 pats}
-             (str : String) (Hlen : length str = 0)
-             (p : pb_productions G valid0 pats)
-             {struct p}
-  : { p : parse_of G str pats
-          & Forall_parse_of (fun _ nt' => is_valid_nonterminal valid0 nt') p }
-  with parse_empty_from_pb_parse_of_production
-         {valid0 pat}
-         (str : String) (Hlen : length str = 0)
-         (p: pb_production G valid0 pat)
-         {struct p}
-       : { p : parse_of_production G str pat
-               & Forall_parse_of_production (fun _ nt' => is_valid_nonterminal valid0 nt') p }.
-  Proof.
-    { destruct p as [ ?? p | ?? p ]; simpl in *.
-      { pose proof (parse_empty_from_pb_parse_of_production valid0 _ _ Hlen p) as p'.
-        eexists (ParseHead _ (projT1 p')).
-        exact (projT2 p'). }
-      { pose proof (parse_empty_from_pb_parse_of_productions valid0 _ _ Hlen p) as p'.
-        eexists (ParseTail _ (projT1 p')).
-        exact (projT2 p'). } }
-    { destruct p as [ | ?? p0 p1 ]; simpl in *.
-      { exists (ParseProductionNil G _ Hlen). constructor. }
-      { eapply (@parse_empty_from_pb_parse_of_item' parse_empty_from_pb_parse_of_productions) in p0.
-        eapply (@parse_empty_from_pb_parse_of_production) in p1.
-        { eexists (ParseProductionCons _ 0 (projT1 p0) (projT1 p1)).
-          exact (projT2 p0, projT2 p1). }
-        { rewrite ?take_length, ?drop_length, Hlen; reflexivity. }
-        { rewrite ?take_length, ?drop_length, Hlen, Min.min_0_r; reflexivity. } } }
-  Defined.
-
-  Definition parse_empty_from_pb_parse_of_item
+  Definition paren_balanced_from_pb_parse_of_item
              {valid0 it}
              (str : String) (Hlen : length str = 0)
              (p : pb_item G valid0 it)
   : { p : parse_of_item G str it
           & Forall_parse_of_item (fun _ nt' => is_valid_nonterminal valid0 nt') p }
-    := @parse_empty_from_pb_parse_of_item' (@parse_empty_from_pb_parse_of_productions) valid0 it str Hlen p.
+    := @paren_balanced_from_pb_parse_of_item' (@paren_balanced_from_pb_parse_of_productions) valid0 it str Hlen p.
 
-  Definition parse_empty_from_minimal_pb_parse_of_item
+  Definition paren_balanced_from_minimal_pb_parse_of_item
              {valid0 it}
              (str : String) (Hlen : length str = 0)
              (p : minimal_pb_item (G := G) valid0 it)
   : { p : parse_of_item G str it
           & Forall_parse_of_item (fun _ nt' => is_valid_nonterminal valid0 nt') p }.
   Proof.
-    eapply parse_empty_from_pb_parse_of_item; trivial.
+    eapply paren_balanced_from_pb_parse_of_item; trivial.
     eapply pb_item__of__minimal_pb_item; try eassumption; reflexivity.
   Qed.
 
-  Definition parse_empty_from_minimal_pb_parse_of_production
+  Definition paren_balanced_from_minimal_pb_parse_of_production
              {valid0 pat}
              (str : String) (Hlen : length str = 0)
              (p : minimal_pb_production (G := G) valid0 pat)
   : { p : parse_of_production G str pat
           & Forall_parse_of_production (fun _ nt' => is_valid_nonterminal valid0 nt') p }.
   Proof.
-    eapply parse_empty_from_pb_parse_of_production; trivial.
+    eapply paren_balanced_from_pb_parse_of_production; trivial.
     eapply pb_production__of__minimal_pb_production; try eassumption; reflexivity.
   Qed.
 
-  Definition parse_empty_from_minimal_pb_parse_of_productions
+  Definition paren_balanced_from_minimal_pb_parse_of_productions
              {valid0 pats}
              (str : String) (Hlen : length str = 0)
              (p : minimal_pb_productions (G := G) valid0 pats)
   : { p : parse_of G str pats
           & Forall_parse_of (fun _ nt' => is_valid_nonterminal valid0 nt') p }.
   Proof.
-    eapply parse_empty_from_pb_parse_of_productions; trivial.
+    eapply paren_balanced_from_pb_parse_of_productions; trivial.
     eapply pb_productions__of__minimal_pb_productions; try eassumption; reflexivity.
   Qed.
 End cfg.
